coq/proof/SoundReduceMaydiff.v
@@ -15,6 +15,8 @@ Require Import paco.
 Import Opsem.
 
 Require Import TODO.
+Require Import Exprs.
+Require Import Hints.
 Require Import Postcond.
 Require Import Validator.
 Require Import GenericValues.
@@ -23,27 +25,183 @@ Require InvState.
 
 Set Implicit Arguments.
 
-Lemma get_lhs_in_spec
-      ld (rhs: Exprs.Expr.t) x
-  (LHS: Exprs.ExprPairSet.In x (Hints.Invariant.get_lhs ld rhs)):
-  (snd x) = rhs /\ Exprs.ExprPairSet.In x ld.
-Proof.
-  unfold Hints.Invariant.get_lhs, flip in *.
-  rewrite Exprs.ExprPairSetFacts.filter_iff in LHS; cycle 1.
-  { solve_compat_bool. }
-  des. des_sumbool. ss.
-Qed.
 
-Lemma get_rhs_in_spec
-      ld (lhs: Exprs.Expr.t) x
-  (RHS: Exprs.ExprPairSet.In x (Hints.Invariant.get_rhs ld lhs)):
-  (fst x) = lhs /\ Exprs.ExprPairSet.In x ld.
-Proof.
-  unfold Hints.Invariant.get_rhs, flip in *.
-  rewrite Exprs.ExprPairSetFacts.filter_iff in RHS; cycle 1.
-  { solve_compat_bool. }
-  des. des_sumbool. ss.
-Qed.
+Section Filter.
+  Definition filter
+             (preserved: Exprs.Tag.t * id -> bool)
+             (inv: InvState.Unary.t): InvState.Unary.t :=
+    InvState.Unary.update_ghost
+      (filter_AL_atom (preserved <*> (pair Exprs.Tag.ghost)))
+      (InvState.Unary.update_previous
+         (filter_AL_atom (preserved <*> (pair Exprs.Tag.previous)))
+         inv).
+
+  Lemma filter_subset_idT st_unary f id invst_unary val
+        (VAL_SUBSET: (InvState.Unary.sem_idT st_unary (filter f invst_unary) id = Some val)):
+    <<VAL: (InvState.Unary.sem_idT st_unary invst_unary id = Some val)>>.
+  Proof.
+    destruct id. destruct t; ss.
+    - eapply lookup_AL_filter_some. exact VAL_SUBSET.
+    - eapply lookup_AL_filter_some. exact VAL_SUBSET.
+  Qed.
+
+  Lemma filter_subset_valueT conf_unary st_unary f vt invst_unary val
+        (VAL_SUBSET: (InvState.Unary.sem_valueT
+                        conf_unary st_unary
+                        (filter f invst_unary) vt = Some val)):
+    <<VAL: (InvState.Unary.sem_valueT conf_unary st_unary invst_unary vt = Some val)>>.
+  Proof.
+    red. destruct vt; ss.
+    eapply filter_subset_idT; eauto.
+  Qed.
+
+  Lemma filter_subset_list_valueT conf_unary st_unary f vts invst_unary val
+        (VAL_SUBSET: (InvState.Unary.sem_list_valueT
+                        conf_unary st_unary
+                        (filter f invst_unary) vts = Some val)):
+    <<VAL: (InvState.Unary.sem_list_valueT conf_unary st_unary invst_unary vts = Some val)>>.
+  Proof.
+    red. revert val VAL_SUBSET. induction vts; i; ss. destruct a.
+    Ltac exploit_with H x :=
+      (exploit H; [exact x|]; eauto; ii; des).
+    des_ifs; ss;
+      (all_once exploit_with filter_subset_valueT);
+      (exploit IHvts; eauto; i); clarify.
+  Qed.
+
+  Lemma filter_subset_expr conf_unary st_unary f expr invst_unary val
+        (VAL_SUBSET: (InvState.Unary.sem_expr
+                        conf_unary st_unary
+                        (filter f invst_unary) expr = Some val)):
+    <<VAL: (InvState.Unary.sem_expr conf_unary st_unary invst_unary expr = Some val)>>.
+  Proof.
+    red.
+    Ltac exploit_filter_subset_with x :=
+      match (type of x) with
+      | (InvState.Unary.sem_valueT _ _ _ _ = Some _) =>
+        (exploit filter_subset_valueT; [exact x|]; eauto; ii; des)
+      | (InvState.Unary.sem_list_valueT _ _ _ _ = Some _) =>
+        (exploit filter_subset_list_valueT; [exact x|]; eauto; ii; des)
+      end.
+    Time destruct expr; ss;
+      des_ifs; ss; (all_once exploit_filter_subset_with); clarify.
+  (* exploit_with: Finished transaction in 25.39 secs (25.194u,0.213s) (successful) *)
+  (* exploit_with_fast: Finished transaction in 7.575 secs (7.536u,0.044s) (successful) *)
+  Qed.
+
+  Lemma filter_preserved_valueT
+        conf_unary st_unary invst_unary vt val f
+        (VAL: InvState.Unary.sem_valueT conf_unary st_unary invst_unary vt = Some val)
+        (PRESERVED: (sflib.is_true (List.forallb f (Exprs.ValueT.get_idTs vt)))):
+    <<VAL: InvState.Unary.sem_valueT conf_unary st_unary (filter f invst_unary) vt = Some val>>.
+  Proof.
+    red. destruct vt; ss. repeat (des_bool; des).
+    unfold InvState.Unary.sem_idT. destruct x. s.
+    destruct t; ss.
+    - rewrite lookup_AL_filter_spec in *. des_ifs.
+      unfold compose in *. unfold Tag.t in *. clarify.
+    - rewrite lookup_AL_filter_spec in *. des_ifs.
+      unfold compose in *. unfold Tag.t in *. clarify.
+  Qed.
+
+  Lemma filter_preserved_list_valueT
+        conf_unary st_unary invst_unary vts val f
+        (VAL: InvState.Unary.sem_list_valueT conf_unary st_unary invst_unary vts = Some val)
+        (PRESERVED: sflib.is_true (List.forallb
+                                     (fun x => (List.forallb f (Exprs.ValueT.get_idTs x)))
+                                     (List.map snd vts))):
+    <<VAL: InvState.Unary.sem_list_valueT conf_unary st_unary (filter f invst_unary) vts = Some val>>.
+  Proof.
+    revert val VAL PRESERVED. induction vts; i; ss.
+    destruct a. ss. repeat (des_bool; des).
+    des_ifs; ss.
+    - (exploit filter_preserved_valueT; [exact Heq1| |]; eauto; ii; des).
+      exploit IHvts; eauto; []; ii; des. clarify.
+    - (exploit filter_preserved_valueT; [exact Heq1| |]; eauto; ii; des).
+      exploit IHvts; eauto; []; ii; des. clarify.
+    - (exploit filter_preserved_valueT; [exact Heq0| |]; eauto; ii; des).
+      exploit IHvts; eauto; []; ii; des. clarify.
+  Qed.
+
+  Lemma filter_preserved_expr
+        conf_unary st_unary invst_unary expr val f
+        (VAL: InvState.Unary.sem_expr conf_unary st_unary invst_unary expr = Some val)
+        (PRESERVED: List.forallb f (Exprs.Expr.get_idTs expr)):
+    <<VAL: InvState.Unary.sem_expr conf_unary st_unary (filter f invst_unary) expr = Some val>>.
+  Proof.
+    red.
+    unfold Exprs.Expr.get_idTs in *.
+    eapply forallb_filter_map in PRESERVED. des.
+    unfold is_true in PRESERVED. (* des_bool should kill it!!!!!!! KILL ALL is_true *)
+
+    Ltac exploit_filter_preserved_with x :=
+      match (type of x) with
+      | (InvState.Unary.sem_valueT _ _ (filter _ _) _ = _) => fail 1
+      | (InvState.Unary.sem_list_valueT _ _ (filter _ _) _ = _) => fail 1
+      (* Above is REQUIRED in order to prevent inf loop *)
+      | (InvState.Unary.sem_valueT _ _ _ _ = Some _) =>
+        (exploit filter_preserved_valueT; [exact x| |]; eauto; ii; des)
+      | (InvState.Unary.sem_list_valueT _ _ _ _ = Some _) =>
+        (exploit filter_preserved_list_valueT; [exact x| |]; eauto; ii; des)
+      end.
+
+    Time destruct expr; ss;
+      repeat (des_bool; des); des_ifs; clarify;
+        (all_once exploit_filter_subset_with); clarify;
+          (all_once exploit_filter_preserved_with); clarify.
+  Qed.
+
+  Lemma incl_implies_preserved
+        conf st invst0 expr val inv
+        (preserved: _ -> bool)
+        (PRESERVED: forall id (ID: In id (Invariant.get_idTs_unary inv)), preserved id)
+        (VAL: InvState.Unary.sem_expr conf st invst0 expr = Some val)
+        (INCL: incl (Exprs.Expr.get_idTs expr) (Invariant.get_idTs_unary inv)):
+    <<PRESERVED: InvState.Unary.sem_expr conf st (filter preserved invst0) expr = Some val>>.
+  Proof.
+    eapply filter_preserved_expr; eauto. apply forallb_forall. i.
+    apply PRESERVED. apply INCL. ss.
+  Qed.
+
+  Lemma In_map_incl {A} (f: Exprs.ExprPair.t -> list A) x xs
+        (IN: Exprs.ExprPairSet.In x xs):
+    <<IN: List.incl (f x) (List.concat (List.map f (Exprs.ExprPairSet.elements xs)))>>.
+  Proof.
+    apply ExprPairSetFacts.elements_iff in IN. induction IN; ss.
+    - subst. apply incl_appl. apply incl_refl.
+    - apply incl_appr. ss.
+  Qed.
+
+  Lemma filter_spec
+        conf st invst invmem inv
+        (preserved: _ -> bool)
+        (PRESERVED: forall id (ID: In id (Invariant.get_idTs_unary inv)), preserved id)
+        (STATE: InvState.Unary.sem conf st invst invmem inv):
+    InvState.Unary.sem conf st (filter preserved invst) invmem inv.
+  Proof.
+    inv STATE. econs.
+    - ii.
+      exploit filter_subset_expr; eauto. i. des.
+      exploit LESSDEF; eauto. i. des.
+      exploit incl_implies_preserved; eauto.
+      eapply incl_tran; [|eapply incl_tran].
+      + apply incl_appr. apply incl_refl.
+      + eapply In_map_incl in H. des. refine H.
+      + unfold Invariant.get_idTs_unary.
+        apply incl_appl. apply incl_refl.
+    - inv NOALIAS. econs; i.
+      + eapply DIFFBLOCK; eauto.
+        * eapply filter_subset_valueT; eauto.
+        * eapply filter_subset_valueT; eauto.
+      + eapply NOALIAS0; eauto.
+        * eapply filter_subset_valueT; eauto.
+        * eapply filter_subset_valueT; eauto.
+    - ii. exploit UNIQUE; eauto. i. inv x0.
+      econs; eauto.
+    - ii. exploit PRIVATE; eauto.
+      eapply filter_subset_idT; eauto.
+  Qed.
+End Filter.
 
 Lemma reduce_maydiff_lessdef_sound
       m_src m_tgt
@@ -57,15 +215,15 @@ Lemma reduce_maydiff_lessdef_sound
                             (reduce_maydiff_lessdef inv)>>.
 Proof.
   inversion STATE. econs; eauto. ii.
-  ss. rewrite Exprs.IdTSetFacts.filter_b in NOTIN; [|solve_compat_bool].
+  ss. rewrite IdTSetFacts.filter_b in NOTIN; [|solve_compat_bool].
   repeat (des_bool; des); ss; cycle 2.
   { exploit MAYDIFF; eauto. } clear MAYDIFF.
-  apply Exprs.ExprPairSetFacts.exists_iff in NOTIN; [|solve_compat_bool].
+  apply ExprPairSetFacts.exists_iff in NOTIN; [|solve_compat_bool].
   red in NOTIN; des.
-  apply Exprs.ExprPairSetFacts.exists_iff in NOTIN0; [|solve_compat_bool].
+  apply ExprPairSetFacts.exists_iff in NOTIN0; [|solve_compat_bool].
   red in NOTIN0; des.
-  apply get_lhs_in_spec in NOTIN0.
-  apply get_rhs_in_spec in NOTIN.
+  apply InvState.get_lhs_in_spec in NOTIN0.
+  apply InvState.get_rhs_in_spec in NOTIN.
   destruct x, x0. ss. des. subst.
   rename id0 into idt.
 
@@ -94,11 +252,11 @@ Qed.
 Lemma reduce_maydiff_preserved_sem_idT st_src st_tgt
       invst inv id val_src val_tgt
   (VAL_SRC: InvState.Unary.sem_idT st_src
-              (InvState.Unary.filter (reduce_maydiff_preserved inv) (InvState.Rel.src invst)) id =
+              (filter (reduce_maydiff_preserved inv) (InvState.Rel.src invst)) id =
             Some val_src)
   (VAL_TGT: InvState.Unary.sem_idT st_tgt (InvState.Rel.tgt invst) id = Some val_tgt):
   <<VAL_TGT: InvState.Unary.sem_idT st_tgt
-    (InvState.Unary.filter (reduce_maydiff_preserved inv) (InvState.Rel.tgt invst)) id = Some val_tgt>>.
+    (filter (reduce_maydiff_preserved inv) (InvState.Rel.tgt invst)) id = Some val_tgt>>.
 Proof.
   destruct id. rename i0 into id.
   unfold InvState.Unary.sem_idT in *. ss.
@@ -127,14 +285,14 @@ Lemma reduce_maydiff_non_physical_sound
     <<STATE: InvState.Rel.sem conf_src conf_tgt st_src st_tgt invst1 invmem
                               (reduce_maydiff_non_physical inv)>>.
 Proof.
-  exists (InvState.Rel.filter (reduce_maydiff_preserved inv) invst0). red.
+  exists (InvState.Rel.update_both (filter (reduce_maydiff_preserved inv)) invst0). red.
   inv STATE.
   econs; ss; cycle 2.
   - ii. ss.
-    rewrite Exprs.IdTSetFacts.filter_b in NOTIN; [|solve_compat_bool].
+    rewrite IdTSetFacts.filter_b in NOTIN; [|solve_compat_bool].
     des_bool. des.
     + exploit MAYDIFF; eauto.
-      { exploit InvState.Unary.filter_subset_idT; eauto. }
+      { exploit filter_subset_idT; eauto. }
       i. des. esplits; eauto.
       eapply reduce_maydiff_preserved_sem_idT; eauto.
     + destruct id0.
@@ -144,10 +302,10 @@ Proof.
       unfold compose in *.
       destruct __t__; inv NOTIN.
       * rewrite lookup_AL_filter_spec in VAL_SRC.
-        unfold Exprs.Tag.t in *. rewrite H0 in VAL_SRC. ss.
+        unfold Tag.t in *. rewrite H0 in VAL_SRC. ss.
       * rewrite lookup_AL_filter_spec in VAL_SRC.
-        unfold Exprs.Tag.t in *. rewrite H0 in VAL_SRC. ss.
-  - apply InvState.Unary.filter_spec; ss. i.
+        unfold Tag.t in *. rewrite H0 in VAL_SRC. ss.
+  - apply filter_spec; ss. i.
     unfold reduce_maydiff_preserved. apply orb_true_iff. right.
     rewrite find_app.
     match goal with
@@ -156,8 +314,8 @@ Proof.
       destruct g eqn:COND
     end; ss.
     eapply find_none in COND; [|eauto].
-    destruct (Exprs.IdT.eq_dec id0 id0); ss.
-  - apply InvState.Unary.filter_spec; ss. i.
+    destruct (IdT.eq_dec id0 id0); ss.
+  - apply filter_spec; ss. i.
     unfold reduce_maydiff_preserved. apply orb_true_iff. right.
     rewrite find_app.
     match goal with
